Examples/riscv_collatz_smc_proof.v
@@ -1,0 +1,84 @@
+Require Import Picinae_theory.
+Require Import riscv_collatz_smc.
+Require Import Picinae_riscv.
+Require Import NArith.
+Require Import Lia ZifyN ZifyBool.
+
+Import RISCVNotations.
+
+Definition collatz_start : N :=  0x100.
+Definition collatz_end   : N :=  0x100 + 4 * 10.
+
+Section Invariants.
+  Variables inp : N.
+  Variable  s0 : store.
+
+  Definition postcondition (s:store) :=
+    s R_A0 = if N.even inp then inp >> 1 else inp ⊕ (1 ⊕ inp >> 1).
+  Definition mem_unchanged (s:store) := s0 V_MEM32 = s V_MEM32 /\ s0 A_EXEC = s A_EXEC.
+  Definition invs (t:trace) : option Prop:=
+    match t with (Addr a, s) :: _ => match a with
+      | 0x100 => Some (mem_unchanged s /\ s R_A0 = inp)
+      | 0x124 => Some (postcondition s)
+      | _ => None end
+    | _ => None end.
+End Invariants.
+
+Definition collatz_exit (t:trace) :=
+  match t with (Addr a,_)::_ => match a with
+  | 0x124 => true
+  | _ => false
+  end | _ => false end.
+
+Theorem collatz_correctness:
+  forall s t s' x' inp
+         (ENTRY: startof t (x',s') = (Addr 0x100,s))
+         (MDL: models rvtypctx s)
+         (INP: s R_A0 = inp)
+         (MEM: collatz_riscv s)
+         (EXEC: collatz_riscv_aexec (s A_EXEC))
+,
+(* We define our program as rv_prog, a function that looks into
+   a given store's memory and page-execute permissions to determine
+   what the next instruction is.
+   Above we specified that the memory of the initial store is exactly
+   our program, which is held in bytes 0-12 with all other bytes 0.
+*)
+  satisfies_all rv_prog (invs inp s) collatz_exit ((x',s')::t).
+Proof.
+Local Ltac step := time ISA_step.
+intros. unfold satisfies_all.
+  apply prove_invs.
+  (* Base case: *)
+  simpl. rewrite ENTRY.
+  step. repeat (split; try assumption).
+
+  intros.
+  erewrite startof_prefix in ENTRY; try eassumption.
+  eapply models_at_invariant; try (eassumption || apply welltyped_rvprog).
+  clear MDL; intros MDL.
+  clear - PRE MDL MEM EXEC. rename s into s0, t1 into t, s1 into s.
+
+  destruct_inv 32 PRE.
+  destruct PRE as ((MEMSAME & EXECSAME) & INP).
+  unfold collatz_riscv, collatz_riscv_aexec in *; rewrite MEMSAME, EXECSAME in *.
+  clear MEMSAME EXECSAME.
+
+  step.
+  step.
+  step.
+  step.
+  step.
+  step.
+  step.
+  step.
+
+  assert (inp mod 2 < 2) by lia.
+  destruct (inp mod 2) as [|p] eqn:EQ; try destruct p; try lia.
+
+  step.
+  admit.
+
+  step.
+  admit.
+Admitted.
